WIP

NuPrime.thy
@@ -8,19 +8,16 @@ theory NuPrime \<comment> \<open>The Primary Theory of the \<nu>-System\<close>
       and "<and>" = "\<^bold>a\<^bold>n\<^bold>d"
       and "in" = "\<^bold>i\<^bold>n"
       and "<with>" = "\<^bold>w\<^bold>i\<^bold>t\<^bold>h"
-      and "auxiliary_facts" = "\<^bold>w\<^bold>i\<^bold>t\<^bold>h \<^bold>f\<^bold>a\<^bold>c\<^bold>t\<^bold>s"
-      and "auxfacts" = "\<^bold>w\<^bold>i\<^bold>t\<^bold>h \<^bold>f\<^bold>a\<^bold>c\<^bold>t\<^bold>s"
+      and "<facts>" = "\<^bold>f\<^bold>a\<^bold>c\<^bold>t\<^bold>s"
       and "<proc>" = "\<^bold>p\<^bold>r\<^bold>o\<^bold>c"
       and "<map>" = "\<^bold>m\<^bold>a\<^bold>p"
       and "<param>" = "\<^bold>p\<^bold>a\<^bold>r\<^bold>a\<^bold>m"
       and ",," = "\<heavy_comma>"
       and "<cast>" = "\<^bold>c\<^bold>a\<^bold>s\<^bold>t"
-      and "<claim>" = "\<^bold>c\<^bold>l\<^bold>a\<^bold>i\<^bold>m"
       and "<conversion>" = "\<^bold>c\<^bold>o\<^bold>n\<^bold>v\<^bold>e\<^bold>r\<^bold>s\<^bold>i\<^bold>o\<^bold>n"
       and "<auto>" = "\<^bold>a\<^bold>u\<^bold>t\<^bold>o"
       and "<premise>" = "\<^bold>p\<^bold>r\<^bold>e\<^bold>m\<^bold>i\<^bold>s\<^bold>e"
-      and atomic = "\<^bold>a\<^bold>t\<^bold>o\<^bold>m\<^bold>i\<^bold>c"
-      and construct = "\<^bold>c\<^bold>o\<^bold>n\<^bold>s\<^bold>t\<^bold>r\<^bold>u\<^bold>c\<^bold>t"
+      and "<construct>" = "\<^bold>c\<^bold>o\<^bold>n\<^bold>s\<^bold>t\<^bold>r\<^bold>u\<^bold>c\<^bold>t"
       and "by" = "\<^bold>b\<^bold>y"
       and "<simplify>" = "\<^bold>s\<^bold>i\<^bold>m\<^bold>p\<^bold>l\<^bold>i\<^bold>f\<^bold>y"
       and "<END>" = "\<^bold>E\<^bold>N\<^bold>D"
@@ -30,6 +27,7 @@ theory NuPrime \<comment> \<open>The Primary Theory of the \<nu>-System\<close>
       and "<when>" = "\<^bold>w\<^bold>h\<^bold>e\<^bold>n"
       and "<intro>" = "\<^bold>i\<^bold>n\<^bold>t\<^bold>r\<^bold>o"
       and "<dest>" = "\<^bold>d\<^bold>e\<^bold>s\<^bold>t"
+      and "<try>" = "\<^bold>t\<^bold>r\<^bold>y"
 begin
 
 text \<open>The fundamental theory for \<nu>-system\<close>
@@ -40,12 +38,13 @@ ML_file NuConfig.ML
 bundle show_more1 = [[show_hyps = true, show_types = true, show_sorts = true]]
 bundle show_more = [[show_hyps = true, show_types = true]]
 
-named_theorems \<nu>intro "\<nu>-type introduction rules" and \<nu>intro' and \<nu>intro0 and \<nu>elim "\<nu>-type elimination rules"
-  \<comment> \<open>\<nu> introduction and elimination rules destructs and reconstructs \<nu> typings.
-    They are not required in the program construction,
-    and generally it is not expected to destruct \<nu> typings during the construction.
-    Therefore, they are not included in the standard introduction and elimination rules.
-    However they are quite useful in primitive proofs for properties (e.g. cast) and instructions. \<close>
+named_theorems \<nu>intro0 "\<nu> auto reasoning rules - highest priority"
+  and \<nu>intro "\<nu> auto reasoning rules - normal priority"
+  and \<nu>intro' "\<nu> auto reasoning rules - low priority"
+  and \<nu>intro'' "\<nu> auto reasoning rules - lowest priority"
+  \<comment> \<open>Prioritized introduction rules. No rule of lower priority will be applied unless all rules of
+    higher priority are attempted. \<close>
+named_theorems \<nu>elim "\<nu>-type elimination rules"
 named_theorems \<nu>def \<open>primitive definitions used to unfold in proofs of primitive instructions.\<close>
   (* and \<nu>address_def \<open>primitive definitions for unfolding in proofs for address\<close> *)
   and \<nu>post_construct and \<nu>auto_destruct
@@ -280,7 +279,9 @@ lemma [elim!,\<nu>elim]: "\<^bold>p\<^bold>a\<^bold>r\<^bold>a\<^bold>m x \<Long
 subsubsection \<open>Premise tag\<close>
 
 definition Premise :: "bool \<Rightarrow> bool" ("\<^bold>p\<^bold>r\<^bold>e\<^bold>m\<^bold>i\<^bold>s\<^bold>e _" [27] 26) where [\<nu>def]:"Premise x = x"
-  \<comment> \<open>A tag to hint automatic provers to try to prove this proof obligation\<close>
+  \<comment> \<open>The tag represent a necessary premise that must be solved in a rule or procedure.
+    The automatic reasoning ties to solve it, and if fails, terminates the automatic reasoning.\<close>
+
 lemma Premise_I: "P \<Longrightarrow> \<^bold>p\<^bold>r\<^bold>e\<^bold>m\<^bold>i\<^bold>s\<^bold>e P" unfolding Premise_def by simp
 lemma Premise_E: "\<^bold>p\<^bold>r\<^bold>e\<^bold>m\<^bold>i\<^bold>s\<^bold>e P \<Longrightarrow> P" unfolding Premise_def by simp
 lemma [elim!,\<nu>elim]: "\<^bold>p\<^bold>r\<^bold>e\<^bold>m\<^bold>i\<^bold>s\<^bold>e P \<Longrightarrow> (P \<Longrightarrow> C) \<Longrightarrow> C" unfolding Premise_def by simp
@@ -301,8 +302,16 @@ lemma Simplify_I: "y \<equiv> x \<Longrightarrow> \<^bold>s\<^bold>i\<^bold>m\<^
 
 subsubsection \<open>Intro and Dest tag\<close>
 
-definition Intro :: " bool \<Rightarrow> bool " ("\<^bold>i\<^bold>n\<^bold>t\<^bold>r\<^bold>o _") where "Intro P = P"
-definition Dest :: " bool \<Rightarrow> bool " ("\<^bold>d\<^bold>e\<^bold>s\<^bold>t _") where "Dest P = P"
+definition Intro :: " bool \<Rightarrow> bool " ("\<^bold>i\<^bold>n\<^bold>t\<^bold>r\<^bold>o _" [12] 11) where "Intro P = P"
+definition Dest :: " bool \<Rightarrow> bool " ("\<^bold>d\<^bold>e\<^bold>s\<^bold>t _" [12] 11) where "Dest P = P"
+
+subsubsection \<open>Different tag\<close>
+
+definition Different :: " 'a \<Rightarrow> 'a \<Rightarrow> bool " where "Different A B = True"
+  \<comment> \<open>A premise that solved by automatic reasoning only if the term expressions of A and B
+  are not alpha-equivalent. It is useful to break up the self-loop. For example,
+  while the introduction rule `cast A \<longmapsto> B \<Longrightarrow> cast B \<longmapsto> C \<Longrightarrow> cast A \<longmapsto> C` causes loop if given `cast A \<longmapsto> A`,
+  the rule `cast A \<longmapsto> B \<Longrightarrow> Different A B \<Longrightarrow> cast B \<longmapsto> C \<Longrightarrow> cast A \<longmapsto> C` will not.\<close>
 
 subsection \<open>Register and its collection\<close>
 
@@ -679,28 +688,34 @@ lemma move_fact_to_star2[simp]:
 
   subsection \<open>Cast\<close>
 
-definition Cast :: " 'a set \<Rightarrow> 'a set \<Rightarrow> bool \<Rightarrow> bool " ("(2\<^bold>c\<^bold>a\<^bold>s\<^bold>t _ \<longmapsto> _/ \<^bold>w\<^bold>i\<^bold>t\<^bold>h _)" [2,2,14] 13)
-  where "(\<^bold>c\<^bold>a\<^bold>s\<^bold>t A \<longmapsto> B \<^bold>w\<^bold>i\<^bold>t\<^bold>h P) \<longleftrightarrow> (\<forall>x. x \<in> A \<longrightarrow> x \<in> B \<and> P)"
-consts SimpleCast :: " 'a set \<Rightarrow> 'a set \<Rightarrow> bool " ("(2\<^bold>c\<^bold>a\<^bold>s\<^bold>t _/ \<longmapsto> _)" [2,14] 13)
-translations "(\<^bold>c\<^bold>a\<^bold>s\<^bold>t A \<longmapsto> B)" == "(\<^bold>c\<^bold>a\<^bold>s\<^bold>t A \<longmapsto> B \<^bold>w\<^bold>i\<^bold>t\<^bold>h CONST True)"
+definition Cast :: " 'a set \<Rightarrow> 'a set \<Rightarrow> bool \<Rightarrow> bool \<Rightarrow> bool " ("(2\<^bold>c\<^bold>a\<^bold>s\<^bold>t _ \<longmapsto> _/ \<^bold>w\<^bold>i\<^bold>t\<^bold>h _ \<^bold>w\<^bold>h\<^bold>e\<^bold>n _)" [13,13,13,13] 12)
+  where "(\<^bold>c\<^bold>a\<^bold>s\<^bold>t A \<longmapsto> B \<^bold>w\<^bold>i\<^bold>t\<^bold>h P \<^bold>w\<^bold>h\<^bold>e\<^bold>n Q) \<longleftrightarrow> (\<forall>v. Q \<longrightarrow> v \<in> A \<longrightarrow> v \<in> B \<and> P)"
+consts SimpleCast1 :: " 'a set \<Rightarrow> 'a set \<Rightarrow> bool \<Rightarrow> bool " ("(2\<^bold>c\<^bold>a\<^bold>s\<^bold>t _/ \<longmapsto> _ \<^bold>w\<^bold>i\<^bold>t\<^bold>h _)" [13,13,13] 12)
+consts SimpleCast2 :: " 'a set \<Rightarrow> 'a set \<Rightarrow> bool \<Rightarrow> bool " ("(2\<^bold>c\<^bold>a\<^bold>s\<^bold>t _/ \<longmapsto> _ \<^bold>w\<^bold>h\<^bold>e\<^bold>n _)" [13,13,13] 12)
+consts SimpleCast3 :: " 'a set \<Rightarrow> 'a set \<Rightarrow> bool " ("(2\<^bold>c\<^bold>a\<^bold>s\<^bold>t _/ \<longmapsto> _)" [13,13] 12)
+translations
+  "(\<^bold>c\<^bold>a\<^bold>s\<^bold>t A \<longmapsto> B)" == "(\<^bold>c\<^bold>a\<^bold>s\<^bold>t A \<longmapsto> B \<^bold>w\<^bold>i\<^bold>t\<^bold>h CONST True \<^bold>w\<^bold>h\<^bold>e\<^bold>n CONST True)"
+  "(\<^bold>c\<^bold>a\<^bold>s\<^bold>t A \<longmapsto> B \<^bold>w\<^bold>i\<^bold>t\<^bold>h P)" == "(\<^bold>c\<^bold>a\<^bold>s\<^bold>t A \<longmapsto> B \<^bold>w\<^bold>i\<^bold>t\<^bold>h P \<^bold>w\<^bold>h\<^bold>e\<^bold>n CONST True)"
+  "(\<^bold>c\<^bold>a\<^bold>s\<^bold>t A \<longmapsto> B \<^bold>w\<^bold>h\<^bold>e\<^bold>n P)" == "(\<^bold>c\<^bold>a\<^bold>s\<^bold>t A \<longmapsto> B \<^bold>w\<^bold>i\<^bold>t\<^bold>h CONST True \<^bold>w\<^bold>h\<^bold>e\<^bold>n P)"
 
-
-definition CastDual :: " 'a set \<Rightarrow> 'a set \<Rightarrow> bool \<Rightarrow> 'b set \<Rightarrow> 'b set \<Rightarrow> bool \<Rightarrow> bool " ("(2\<^bold>c\<^bold>a\<^bold>s\<^bold>t _/ \<longmapsto> _/ \<^bold>w\<^bold>i\<^bold>t\<^bold>h _/ \<^bold>d\<^bold>u\<^bold>a\<^bold>l _/ \<longmapsto> _/ \<^bold>w\<^bold>h\<^bold>e\<^bold>n _)" [2,2,2,2,14] 13)
-  where "CastDual A B P A' B' P' \<longleftrightarrow> (\<^bold>c\<^bold>a\<^bold>s\<^bold>t A \<longmapsto> B \<^bold>w\<^bold>i\<^bold>t\<^bold>h P) \<and> (P' \<longrightarrow> (\<^bold>c\<^bold>a\<^bold>s\<^bold>t A' \<longmapsto> B'))"
-consts SimpCastDual1 :: " 'a set \<Rightarrow> 'a set \<Rightarrow> 'b set \<Rightarrow> 'b set \<Rightarrow> bool \<Rightarrow> bool " ("(2\<^bold>c\<^bold>a\<^bold>s\<^bold>t _/ \<longmapsto> _/ \<^bold>d\<^bold>u\<^bold>a\<^bold>l _/ \<longmapsto> _/ \<^bold>w\<^bold>h\<^bold>e\<^bold>n _)" [2,2,2,14] 13)
-consts SimpCastDual2 :: " 'a set \<Rightarrow> 'a set \<Rightarrow> bool \<Rightarrow> 'b set \<Rightarrow> 'b set \<Rightarrow> bool " ("(2\<^bold>c\<^bold>a\<^bold>s\<^bold>t _/ \<longmapsto> _/ \<^bold>w\<^bold>i\<^bold>t\<^bold>h _/ \<^bold>d\<^bold>u\<^bold>a\<^bold>l _/ \<longmapsto> _)" [2,2,2,14] 13)
-consts SimpCastDual3 :: " 'a set \<Rightarrow> 'a set \<Rightarrow> 'b set \<Rightarrow> 'b set \<Rightarrow> bool " ("(2\<^bold>c\<^bold>a\<^bold>s\<^bold>t _/ \<longmapsto> _/ \<^bold>d\<^bold>u\<^bold>a\<^bold>l _/ \<longmapsto> _)" [2,2,14] 13)
+definition CastDual :: " 'a set \<Rightarrow> 'a set \<Rightarrow> bool \<Rightarrow> 'b set \<Rightarrow> 'b set \<Rightarrow> bool \<Rightarrow> bool " ("(2\<^bold>c\<^bold>a\<^bold>s\<^bold>t _/ \<longmapsto> _/ \<^bold>w\<^bold>i\<^bold>t\<^bold>h _/ \<^bold>d\<^bold>u\<^bold>a\<^bold>l _/ \<longmapsto> _/ \<^bold>w\<^bold>h\<^bold>e\<^bold>n _)" [13,13,13,13,13] 12)
+  where "CastDual A B P A' B' P' \<longleftrightarrow> (\<^bold>c\<^bold>a\<^bold>s\<^bold>t A \<longmapsto> B \<^bold>w\<^bold>i\<^bold>t\<^bold>h P) \<and> (\<^bold>c\<^bold>a\<^bold>s\<^bold>t A' \<longmapsto> B' \<^bold>w\<^bold>h\<^bold>e\<^bold>n P')"
+consts SimpCastDual1 :: " 'a set \<Rightarrow> 'a set \<Rightarrow> 'b set \<Rightarrow> 'b set \<Rightarrow> bool \<Rightarrow> bool " ("(2\<^bold>c\<^bold>a\<^bold>s\<^bold>t _/ \<longmapsto> _/ \<^bold>d\<^bold>u\<^bold>a\<^bold>l _/ \<longmapsto> _/ \<^bold>w\<^bold>h\<^bold>e\<^bold>n _)" [13,13,13,13] 12)
+consts SimpCastDual2 :: " 'a set \<Rightarrow> 'a set \<Rightarrow> bool \<Rightarrow> 'b set \<Rightarrow> 'b set \<Rightarrow> bool " ("(2\<^bold>c\<^bold>a\<^bold>s\<^bold>t _/ \<longmapsto> _/ \<^bold>w\<^bold>i\<^bold>t\<^bold>h _/ \<^bold>d\<^bold>u\<^bold>a\<^bold>l _/ \<longmapsto> _)" [13,13,13,13] 12)
+consts SimpCastDual3 :: " 'a set \<Rightarrow> 'a set \<Rightarrow> 'b set \<Rightarrow> 'b set \<Rightarrow> bool " ("(2\<^bold>c\<^bold>a\<^bold>s\<^bold>t _/ \<longmapsto> _/ \<^bold>d\<^bold>u\<^bold>a\<^bold>l _/ \<longmapsto> _)" [13,13,13] 12)
 translations
   "\<^bold>c\<^bold>a\<^bold>s\<^bold>t A \<longmapsto> A' \<^bold>d\<^bold>u\<^bold>a\<^bold>l B \<longmapsto> B'" == "\<^bold>c\<^bold>a\<^bold>s\<^bold>t A \<longmapsto> A' \<^bold>w\<^bold>i\<^bold>t\<^bold>h CONST True \<^bold>d\<^bold>u\<^bold>a\<^bold>l B \<longmapsto> B' \<^bold>w\<^bold>h\<^bold>e\<^bold>n CONST True"
   "\<^bold>c\<^bold>a\<^bold>s\<^bold>t A \<longmapsto> A' \<^bold>d\<^bold>u\<^bold>a\<^bold>l B \<longmapsto> B' \<^bold>w\<^bold>h\<^bold>e\<^bold>n Q" == "\<^bold>c\<^bold>a\<^bold>s\<^bold>t A \<longmapsto> A' \<^bold>w\<^bold>i\<^bold>t\<^bold>h CONST True \<^bold>d\<^bold>u\<^bold>a\<^bold>l B \<longmapsto> B' \<^bold>w\<^bold>h\<^bold>e\<^bold>n Q"
   "\<^bold>c\<^bold>a\<^bold>s\<^bold>t A \<longmapsto> A' \<^bold>w\<^bold>i\<^bold>t\<^bold>h P \<^bold>d\<^bold>u\<^bold>a\<^bold>l B \<longmapsto> B'" == "\<^bold>c\<^bold>a\<^bold>s\<^bold>t A \<longmapsto> A' \<^bold>w\<^bold>i\<^bold>t\<^bold>h P \<^bold>d\<^bold>u\<^bold>a\<^bold>l B \<longmapsto> B' \<^bold>w\<^bold>h\<^bold>e\<^bold>n CONST True"
 
-translations "\<^bold>c\<^bold>a\<^bold>s\<^bold>t x \<tycolon> X \<longmapsto> B \<^bold>w\<^bold>i\<^bold>t\<^bold>h P" == "\<^bold>c\<^bold>a\<^bold>s\<^bold>t \<tort_lbrace> x \<tycolon> X \<tort_rbrace> \<longmapsto> B \<^bold>w\<^bold>i\<^bold>t\<^bold>h P"
-  "\<^bold>c\<^bold>a\<^bold>s\<^bold>t A \<longmapsto> x \<tycolon> X \<^bold>w\<^bold>i\<^bold>t\<^bold>h P" == "\<^bold>c\<^bold>a\<^bold>s\<^bold>t A \<longmapsto> \<tort_lbrace> x \<tycolon> X \<tort_rbrace> \<^bold>w\<^bold>i\<^bold>t\<^bold>h P"
+translations
+  "\<^bold>c\<^bold>a\<^bold>s\<^bold>t x \<tycolon> X \<longmapsto> B \<^bold>w\<^bold>i\<^bold>t\<^bold>h P \<^bold>w\<^bold>h\<^bold>e\<^bold>n Q" == "\<^bold>c\<^bold>a\<^bold>s\<^bold>t \<tort_lbrace> x \<tycolon> X \<tort_rbrace> \<longmapsto> B \<^bold>w\<^bold>i\<^bold>t\<^bold>h P \<^bold>w\<^bold>h\<^bold>e\<^bold>n Q"
+  "\<^bold>c\<^bold>a\<^bold>s\<^bold>t A \<longmapsto> x \<tycolon> X \<^bold>w\<^bold>i\<^bold>t\<^bold>h P \<^bold>w\<^bold>h\<^bold>e\<^bold>n Q" == "\<^bold>c\<^bold>a\<^bold>s\<^bold>t A \<longmapsto> \<tort_lbrace> x \<tycolon> X \<tort_rbrace> \<^bold>w\<^bold>i\<^bold>t\<^bold>h P \<^bold>w\<^bold>h\<^bold>e\<^bold>n Q"
   "\<^bold>c\<^bold>a\<^bold>s\<^bold>t A \<longmapsto> x \<tycolon> X \<^bold>w\<^bold>i\<^bold>t\<^bold>h P' \<^bold>d\<^bold>u\<^bold>a\<^bold>l A' \<longmapsto> B' \<^bold>w\<^bold>h\<^bold>e\<^bold>n P" == "\<^bold>c\<^bold>a\<^bold>s\<^bold>t A \<longmapsto> \<tort_lbrace>x \<tycolon> X\<tort_rbrace> \<^bold>w\<^bold>i\<^bold>t\<^bold>h P' \<^bold>d\<^bold>u\<^bold>a\<^bold>l A' \<longmapsto> B' \<^bold>w\<^bold>h\<^bold>e\<^bold>n P"
   "\<^bold>c\<^bold>a\<^bold>s\<^bold>t a \<tycolon> A \<longmapsto> B \<^bold>w\<^bold>i\<^bold>t\<^bold>h P' \<^bold>d\<^bold>u\<^bold>a\<^bold>l A' \<longmapsto> B' \<^bold>w\<^bold>h\<^bold>e\<^bold>n P" == "\<^bold>c\<^bold>a\<^bold>s\<^bold>t \<tort_lbrace>a \<tycolon> A\<tort_rbrace> \<longmapsto> B \<^bold>w\<^bold>i\<^bold>t\<^bold>h P' \<^bold>d\<^bold>u\<^bold>a\<^bold>l A' \<longmapsto> B' \<^bold>w\<^bold>h\<^bold>e\<^bold>n P"
   "\<^bold>c\<^bold>a\<^bold>s\<^bold>t A \<longmapsto> B \<^bold>w\<^bold>i\<^bold>t\<^bold>h P' \<^bold>d\<^bold>u\<^bold>a\<^bold>l a' \<tycolon> A' \<longmapsto> B' \<^bold>w\<^bold>h\<^bold>e\<^bold>n P" == "\<^bold>c\<^bold>a\<^bold>s\<^bold>t A \<longmapsto> B \<^bold>w\<^bold>i\<^bold>t\<^bold>h P' \<^bold>d\<^bold>u\<^bold>a\<^bold>l \<tort_lbrace>a' \<tycolon> A'\<tort_rbrace> \<longmapsto> B' \<^bold>w\<^bold>h\<^bold>e\<^bold>n P"
   "\<^bold>c\<^bold>a\<^bold>s\<^bold>t A \<longmapsto> B \<^bold>w\<^bold>i\<^bold>t\<^bold>h P' \<^bold>d\<^bold>u\<^bold>a\<^bold>l A' \<longmapsto> b' \<tycolon> B' \<^bold>w\<^bold>h\<^bold>e\<^bold>n P" == "\<^bold>c\<^bold>a\<^bold>s\<^bold>t A \<longmapsto> B \<^bold>w\<^bold>i\<^bold>t\<^bold>h P' \<^bold>d\<^bold>u\<^bold>a\<^bold>l A' \<longmapsto> \<tort_lbrace>b' \<tycolon> B'\<tort_rbrace> \<^bold>w\<^bold>h\<^bold>e\<^bold>n P"
+
 
 (* abbreviation SimpleCast :: " 'a set \<Rightarrow> 'a set \<Rightarrow> bool " ("(2\<^bold>c\<^bold>a\<^bold>s\<^bold>t _ \<longmapsto> _)" [2,14] 13)
   where "(\<^bold>c\<^bold>a\<^bold>s\<^bold>t A \<longmapsto> B) \<equiv> (\<^bold>c\<^bold>a\<^bold>s\<^bold>t A \<longmapsto> B \<^bold>w\<^bold>i\<^bold>t\<^bold>h True)" *)
@@ -723,7 +738,7 @@ lemma cast_trans: "\<^bold>c\<^bold>a\<^bold>s\<^bold>t A \<longmapsto> B \<^bol
 
 theorem apply_cast: "(\<^bold>c\<^bold>u\<^bold>r\<^bold>r\<^bold>e\<^bold>n\<^bold>t blk \<^bold>r\<^bold>e\<^bold>s\<^bold>u\<^bold>l\<^bold>t\<^bold>s \<^bold>i\<^bold>n (R \<heavy_comma> X\<heavy_comma> \<^bold>h\<^bold>e\<^bold>a\<^bold>p H)) \<Longrightarrow> (\<^bold>c\<^bold>a\<^bold>s\<^bold>t X \<longmapsto> Y \<^bold>w\<^bold>i\<^bold>t\<^bold>h P) \<Longrightarrow> (\<^bold>c\<^bold>u\<^bold>r\<^bold>r\<^bold>e\<^bold>n\<^bold>t blk \<^bold>r\<^bold>e\<^bold>s\<^bold>u\<^bold>l\<^bold>t\<^bold>s \<^bold>i\<^bold>n (R \<heavy_comma> Y\<heavy_comma> \<^bold>h\<^bold>e\<^bold>a\<^bold>p H) \<addition> P)"
   unfolding Procedure_def CurrentConstruction_def PendingConstruction_def bind_def SpecTop_imp Cast_def by (auto 4 6)
-theorem cast: "\<^bold>c\<^bold>u\<^bold>r\<^bold>r\<^bold>e\<^bold>n\<^bold>t blk \<^bold>r\<^bold>e\<^bold>s\<^bold>u\<^bold>l\<^bold>t\<^bold>s \<^bold>i\<^bold>n T \<Longrightarrow> \<^bold>c\<^bold>a\<^bold>s\<^bold>t T \<longmapsto> T' \<^bold>w\<^bold>i\<^bold>t\<^bold>h P \<Longrightarrow> \<^bold>c\<^bold>u\<^bold>r\<^bold>r\<^bold>e\<^bold>n\<^bold>t blk \<^bold>r\<^bold>e\<^bold>s\<^bold>u\<^bold>l\<^bold>t\<^bold>s \<^bold>i\<^bold>n T' "
+theorem cast: "\<^bold>c\<^bold>u\<^bold>r\<^bold>r\<^bold>e\<^bold>n\<^bold>t blk \<^bold>r\<^bold>e\<^bold>s\<^bold>u\<^bold>l\<^bold>t\<^bold>s \<^bold>i\<^bold>n T \<Longrightarrow> \<^bold>c\<^bold>a\<^bold>s\<^bold>t T \<longmapsto> T' \<^bold>w\<^bold>i\<^bold>t\<^bold>h P \<^bold>w\<^bold>h\<^bold>e\<^bold>n Q \<Longrightarrow> \<^bold>p\<^bold>r\<^bold>e\<^bold>m\<^bold>i\<^bold>s\<^bold>e Q \<Longrightarrow> \<^bold>c\<^bold>u\<^bold>r\<^bold>r\<^bold>e\<^bold>n\<^bold>t blk \<^bold>r\<^bold>e\<^bold>s\<^bold>u\<^bold>l\<^bold>t\<^bold>s \<^bold>i\<^bold>n T' "
   for T' :: "(heap \<times> 'a::lrep) set" unfolding Cast_def CurrentConstruction_def by auto
 
 (* theorem proc_cast': "\<^bold>p\<^bold>r\<^bold>o\<^bold>c f \<blangle> A \<longmapsto> B \<brangle> \<Longrightarrow> \<^bold>c\<^bold>a\<^bold>s\<^bold>t A' \<longmapsto> A \<^bold>w\<^bold>i\<^bold>t\<^bold>h P \<Longrightarrow> \<^bold>c\<^bold>a\<^bold>s\<^bold>t B \<longmapsto> B' \<^bold>w\<^bold>i\<^bold>t\<^bold>h Q \<Longrightarrow> \<^bold>p\<^bold>r\<^bold>o\<^bold>c f \<blangle> A' \<longmapsto> B' \<brangle>"
@@ -731,6 +746,14 @@ theorem cast: "\<^bold>c\<^bold>u\<^bold>r\<^bold>r\<^bold>e\<^bold>n\<^bold>t b
 
 lemma [\<nu>intro']: "\<^bold>i\<^bold>n\<^bold>t\<^bold>r\<^bold>o \<^bold>c\<^bold>a\<^bold>s\<^bold>t A \<longmapsto> B \<^bold>w\<^bold>i\<^bold>t\<^bold>h P \<Longrightarrow> \<^bold>c\<^bold>a\<^bold>s\<^bold>t A \<longmapsto> B \<^bold>w\<^bold>i\<^bold>t\<^bold>h P" unfolding Intro_def .
 lemma [\<nu>intro']: "\<^bold>d\<^bold>e\<^bold>s\<^bold>t \<^bold>c\<^bold>a\<^bold>s\<^bold>t A \<longmapsto> B \<^bold>w\<^bold>i\<^bold>t\<^bold>h P \<Longrightarrow> \<^bold>c\<^bold>a\<^bold>s\<^bold>t A \<longmapsto> B \<^bold>w\<^bold>i\<^bold>t\<^bold>h P" unfolding Dest_def .
+
+lemma [\<nu>intro'']: "\<^bold>i\<^bold>n\<^bold>t\<^bold>r\<^bold>o \<^bold>c\<^bold>a\<^bold>s\<^bold>t A \<longmapsto> A" unfolding Intro_def using cast_id .
+lemma [\<nu>intro'']: "\<^bold>d\<^bold>e\<^bold>s\<^bold>t \<^bold>c\<^bold>a\<^bold>s\<^bold>t A \<longmapsto> A" unfolding Dest_def using cast_id .
+  \<comment> \<open>All intro-cast or dest-cast involved in the reasoner constitute a directed acyclic graph WITH self-loop.
+    Note the self-loop has the lowest priority, so that the self-loop only be tried ONCE in the whole reasoning
+      (when all other rules cannot be applied), and only longest inference chains (who cannot be extended by
+      any other rules) will be tried by self-loop.
+    \<^term>\<open>Different\<close> can be used to assert the non-self-loop.\<close>
 
 subsection \<open>Conversion\<close>
 
@@ -747,9 +770,9 @@ lemma conversion: "\<^bold>c\<^bold>o\<^bold>n\<^bold>v\<^bold>e\<^bold>r\<^bold
 
 lemma [\<nu>intro0]: "\<^bold>c\<^bold>o\<^bold>n\<^bold>v\<^bold>e\<^bold>r\<^bold>s\<^bold>i\<^bold>o\<^bold>n f \<blangle> U \<longmapsto> V \<brangle> \<long_dobule_mapsto> f \<blangle> U \<longmapsto> V \<brangle>" unfolding Conversion_def by fast
 
-lemma conversion_cast[\<nu>intro]: "\<^bold>c\<^bold>a\<^bold>s\<^bold>t U' \<longmapsto> U \<^bold>w\<^bold>i\<^bold>t\<^bold>h P \<^bold>d\<^bold>u\<^bold>a\<^bold>l V \<longmapsto> V' \<^bold>w\<^bold>h\<^bold>e\<^bold>n Q \<Longrightarrow> (P \<Longrightarrow> Q) \<Longrightarrow> \<^bold>c\<^bold>o\<^bold>n\<^bold>v\<^bold>e\<^bold>r\<^bold>s\<^bold>i\<^bold>o\<^bold>n f \<blangle> U \<longmapsto> V \<brangle> \<long_dobule_mapsto> f \<blangle> U' \<longmapsto> V'\<brangle>"
+lemma conversion_cast[\<nu>intro]: "\<^bold>c\<^bold>a\<^bold>s\<^bold>t U' \<longmapsto> U \<^bold>w\<^bold>i\<^bold>t\<^bold>h P \<^bold>d\<^bold>u\<^bold>a\<^bold>l V \<longmapsto> V' \<^bold>w\<^bold>h\<^bold>e\<^bold>n Q \<Longrightarrow> \<^bold>p\<^bold>r\<^bold>e\<^bold>m\<^bold>i\<^bold>s\<^bold>e (P \<longrightarrow> Q) \<Longrightarrow> \<^bold>c\<^bold>o\<^bold>n\<^bold>v\<^bold>e\<^bold>r\<^bold>s\<^bold>i\<^bold>o\<^bold>n f \<blangle> U \<longmapsto> V \<brangle> \<long_dobule_mapsto> f \<blangle> U' \<longmapsto> V'\<brangle>"
   unfolding Conversion_def Procedure_def Cast_def CastDual_def id_def
-  by (metis Cast_def CurrentConstruction_def LooseStateTy_introByStrict LooseStateTy_upgrade cast)
+  by (metis Cast_def CurrentConstruction_def LooseStateTy_introByStrict LooseStateTy_upgrade Premise_def cast)
 (* lemma [\<nu>intro]: "\<^bold>p\<^bold>r\<^bold>o\<^bold>c g \<blangle> U' \<longmapsto> U \<brangle> \<Longrightarrow> \<^bold>c\<^bold>o\<^bold>n\<^bold>v\<^bold>e\<^bold>r\<^bold>s\<^bold>i\<^bold>o\<^bold>n f \<blangle> U \<longmapsto> V \<brangle> \<long_dobule_mapsto> (g \<nuInstrComp> f) \<blangle> U' \<longmapsto> V\<brangle>"
   unfolding Conversion_def using instr_comp by fast *)
 
